Add index

specIR/SimSIR.v
@@ -48,67 +48,72 @@ Section SEMANTICS.
 Let st_src := (SIR.state owned_heap_src).
 Let st_tgt := (SIR.state owned_heap_tgt).
 
-Inductive _sim_st (sim_st: st_src -> st_tgt -> Prop): st_src -> st_tgt -> Prop :=
+Variable idx: Type.
+Variable ord: idx -> idx -> Prop.
+Hypothesis wf_ord: well_founded ord.
+
+Inductive _sim_st (sim_st: idx -> st_src -> st_tgt -> Prop) (i0: idx): st_src -> st_tgt -> Prop :=
 | sim_st_ret
     oh_src oh_tgt m v
     (O: SO oh_src oh_tgt)
   :
-    _sim_st sim_st (Ret (oh_src, (m, v))) (Ret (oh_tgt, (m, v)))
+    _sim_st sim_st i0 (Ret (oh_src, (m, v))) (Ret (oh_tgt, (m, v)))
 | sim_st_tau
-    i_src
-    i_tgt
-    (SIM: sim_st i_src i_tgt)
+    i1
+    it_src it_tgt
+    (SIM: sim_st i1 it_src it_tgt)
   :
-    _sim_st sim_st (Tau i_src) (Tau i_tgt)
+    _sim_st sim_st i0 (Tau it_src) (Tau it_tgt)
 | sim_st_ecall
+    i1
     sg m vs fptr
     oh_src k_src
     oh_tgt k_tgt
     (O: SO oh_src oh_tgt)
-    (SIM: HProper (SALL !-> sim_st) k_src k_tgt)
+    (SIM: HProper (SALL !-> sim_st i1) k_src k_tgt)
   :
-    _sim_st sim_st
+    _sim_st sim_st i0
              (Vis (subevent _ (ECall sg fptr oh_src m vs)) k_src)
              (Vis (subevent _ (ECall sg fptr oh_tgt m vs)) k_tgt)
 | sim_st_nb
-    i_src k_tgt
+    it_src k_tgt
   :
-    _sim_st sim_st i_src (Vis (subevent _ (ENB)) k_tgt)
+    _sim_st sim_st i0 it_src (Vis (subevent _ (ENB)) k_tgt)
 | sim_st_ub
-    k_src i_tgt
+    k_src it_tgt
   :
-    _sim_st sim_st (Vis (subevent _ (EUB)) k_src) i_tgt
+    _sim_st sim_st i0 (Vis (subevent _ (EUB)) k_src) it_tgt
 | sim_st_choose_src
-    X_src
-    k_src i_tgt
-    (SIM: exists x_src, sim_st (k_src x_src) i_tgt)
+    i1 X_src
+    k_src it_tgt
+    (SIM: exists x_src, sim_st i1 (k_src x_src) it_tgt)
   :
-    _sim_st sim_st
+    _sim_st sim_st i0
             (Vis (subevent _ (EChoose X_src)) k_src)
-            (Tau i_tgt)
+            (Tau it_tgt)
 | sim_st_choose_tgt
-    X_tgt
-    k_tgt i_src
+    i1 X_tgt
+    k_tgt it_src
     (INHAB: inhabited X_tgt)
-    (SIM: forall x_tgt, sim_st i_src (k_tgt x_tgt))
+    (SIM: forall x_tgt, sim_st i1 it_src (k_tgt x_tgt))
   :
-    _sim_st sim_st
-            (Tau i_src)
+    _sim_st sim_st i0
+            (Tau it_src)
             (Vis (subevent _ (EChoose X_tgt)) k_tgt)
 | sim_st_choose_both
-    X_src X_tgt
+    i1 X_src X_tgt
     k_src k_tgt
     (INHAB: inhabited X_tgt)
-    (SIM: forall x_tgt, exists x_src, sim_st (k_src x_src) (k_tgt x_tgt))
+    (SIM: forall x_tgt, exists x_src, sim_st i1 (k_src x_src) (k_tgt x_tgt))
   :
-    _sim_st sim_st
+    _sim_st sim_st i0
             (Vis (subevent _ (EChoose X_src)) k_src)
             (Vis (subevent _ (EChoose X_tgt)) k_tgt)
 .
 
-Definition sim_st: st_src -> st_tgt -> Prop := paco2 _sim_st bot2.
+Definition sim_st: idx -> st_src -> st_tgt -> Prop := paco3 _sim_st bot3.
 
-Lemma sim_st_mon: monotone2 _sim_st.
+Lemma sim_st_mon: monotone3 _sim_st.
 Proof.
   ii. inv IN; try econs; et.
   - des. esplits; et.
@@ -131,13 +136,17 @@ Hint Resolve sim_st_mon: paco.
 
 Section SIM.
 
+  Variable idx: Type.
+  Variable ord: idx -> idx -> Prop.
+  Hypothesis wf_ord: well_founded ord.
   Variable p_src: program owned_heap_src.
   Variable p_tgt: program owned_heap_tgt.
   Variable sim_prog: forall
       (fname: ident) m vs oh_src oh_tgt
       (O: SO oh_src oh_tgt)
     ,
-      (<<SIM: sim_st (interp_program p_src (ICall fname oh_src m vs))
+      exists (i0: idx),
+      (<<SIM: sim_st i0 (interp_program p_src (ICall fname oh_src m vs))
                      (interp_program p_tgt (ICall fname oh_tgt m vs))
                      >>)
   .
@@ -215,26 +224,26 @@ Section SIM.
     Definition msp: ModSemPair.t := ModSemPair.mk (md_src skenv_link) (md_tgt skenv_link)
                                                   (SimSymbId.mk md_src md_tgt) sm_link.
 
-    Inductive match_states (idx: nat): SIR.state owned_heap_src ->
-                                       SIR.state owned_heap_tgt -> SimMemOh.t -> Prop :=
+    Inductive match_states (i0: idx): SIR.state owned_heap_src ->
+                                      SIR.state owned_heap_tgt -> SimMemOh.t -> Prop :=
     | match_states_intro
         st_src st_tgt smo0
-        (SIM: sim_st st_src st_tgt)
+        (SIM: sim_st i0 st_src st_tgt)
         (MWF: SimMemOh.wf smo0)
       :
-        match_states idx st_src st_tgt smo0
+        match_states i0 st_src st_tgt smo0
     .
 
     Lemma match_states_lxsim
-          idx st_src_src st_tgt_src smo_src
-          (MATCH: match_states idx st_src_src st_tgt_src smo_src)
+          i0 st_src_src st_tgt_src smo_src
+          (MATCH: match_states i0 st_src_src st_tgt_src smo_src)
       :
         <<XSIM: lxsim (md_src skenv_link) (md_tgt skenv_link)
                       (fun _ => () -> exists (_ : ()) (_ : mem), True)
-                      (Ord.lift_idx lt_wf idx) st_src_src st_tgt_src smo_src>>
+                      (Ord.lift_idx wf_ord i0) st_src_src st_tgt_src smo_src>>
     .
     Proof.
-      revert_until idx. revert idx.
+      revert_until i0. revert i0.
       ginit.
       { intros. eapply cpn4_wcompat; eauto with paco. }
       gcofix CIH. i. gstep.
@@ -340,16 +349,18 @@ Section SIM.
       { ii. ss. eexists (mk _ _ _); ss. esplits; eauto. econs; ss; eauto. }
       ii. ss. esplits; eauto.
       - ii. des. inv INITTGT. inv SAFESRC. ss. des_ifs_safe.
-        esplits; eauto.
+        rr in SIMARGS. des. inv SIMARGS0; ss. clarify. inv MWF. ss. destruct sm_arg; ss.
+        destruct sm0; ss. subst. clarify. clear_tac.
+        rename tgt into m0. rename vs_tgt into vs0.
+        exploit (sim_prog fid0 m0 vs0); et. i; des.
+        eexists _, (mk (SimMemId.mk _ _) _ _), _. esplits; eauto.
         { econs; ss; et. }
         eapply match_states_lxsim; eauto.
         econs; ss; et.
-        rr in SIMARGS. des. inv SIMARGS0; ss. clarify. inv MWF. ss. destruct sm_arg; ss.
-        destruct sm0; ss. subst. clarify. clear_tac.
-        assert(fid0 = fid).
-        { apply_all_once Genv.find_invert_symbol. clarify. }
-        clarify.
-        eapply sim_prog; et.
+        + assert(fid0 = fid).
+          { apply_all_once Genv.find_invert_symbol. clarify. }
+          clarify. eauto.
+        + econs; ss; et.
       - i; des. inv SAFESRC. ss. des_ifs.
         rr in SIMARGS. des. inv SIMARGS0; ss. clarify. destruct sm_arg; ss. destruct sm0; ss. clarify.
         esplits; et. econs; ss; et.
